start on clos_to_bvl observational semantics preservation
needed to make the state relation precondition stronger, not sure what
effects this will have further up.

the standard proof does not go through in the divergence case (which is
currently cheated) because clos_to_bvl introduces additional ticks. but
it should hopefully be possible to work around that.

compiler/backend/proofs/clos_to_bvlProofScript.sml
@@ -3703,15 +3703,28 @@ val compile_exps_correct = Q.store_thm("compile_exps_correct",
 
 val full_state_rel_def = Define`
   full_state_rel s1 s2 ⇔
-    ∃sa sb sc sd f.
-      state_rel s1.clock s1 sa ∧ s1.clock = sa.clock ∧
+    ∀k. ∃sa sb sc sd f.
+      state_rel k s1 sa ∧ s1.clock = sa.clock ∧
       clos_numberProof$state_rel sa sb ∧
-      state_rel sb.clock sb sc ∧ sb.clock = sc.clock ∧
+      state_rel k sb sc ∧ sb.clock = sc.clock ∧
       FEVERY (λp. every_Fn_vs_NONE [SND (SND p)]) sc.code ∧
       clos_annotateProof$state_rel sc sd ∧
       FEVERY (λp. every_Fn_vs_SOME [SND (SND p)]) sd.code ∧
       FEVERY (λp. every_Fn_SOME [SND (SND p)]) sd.code ∧
       clos_to_bvlProof$state_rel f sd s2`;
+
+val full_state_rel_with_clock = Q.store_thm("full_state_rel_with_clock",
+  `full_state_rel s1 s2 ⇒ full_state_rel (s1 with clock := k) (s2 with clock := k)`,
+  rw[full_state_rel_def] >>
+  qmatch_goalsub_rename_tac`clos_relation$state_rel ck` >>
+  first_x_assum(qspec_then`ck`strip_assume_tac) >>
+  qexists_tac`sa with clock := k` >> simp[] >>
+  qexists_tac`sb with clock := k` >> simp[] >>
+  qexists_tac`sc with clock := k` >> simp[] >>
+  qexists_tac`sd with clock := k` >> simp[] >>
+  qexists_tac`f`>>simp[] >>
+  fs[clos_numberProofTheory.state_rel_def,
+     clos_annotateProofTheory.state_rel_def]);
 
 val full_result_rel_def = Define`
   full_result_rel (r1,s1) (r2,s2) ⇔
@@ -3727,6 +3740,41 @@ val full_result_rel_def = Define`
       result_rel (LIST_REL clos_numberProof$v_rel) clos_numberProof$v_rel ra rb ∧
       result_rel (LIST_REL clos_annotateProof$v_rel) clos_annotateProof$v_rel rc rd ∧
       result_rel (LIST_REL (v_rel f s2.refs s2.code)) (v_rel f s2.refs s2.code) rd r2`;
+
+val full_result_rel_abort = Q.store_thm("full_result_rel_abort",
+  `r ≠ Rerr(Rabort Rtype_error) ⇒
+  (full_result_rel (r,x) (Rerr (Rabort a),y) ⇒ r = Rerr (Rabort a))`,
+  rw[full_result_rel_def] >>
+  Cases_on`rb`>> fs[clos_relationTheory.res_rel_rw]>>
+  Cases_on`e`>> fs[clos_relationTheory.res_rel_rw]>>
+  Cases_on`r`>> fs[clos_relationTheory.res_rel_rw]>>
+  Cases_on`e`>> fs[clos_relationTheory.res_rel_rw]>>
+  qcase_tac`err = Rabort ac` >>
+  qcase_tac`ab = a` >>
+  Cases_on`ab`>> fs[clos_relationTheory.res_rel_rw]>>
+  Cases_on`ac`>> fs[clos_relationTheory.res_rel_rw]);
+
+val full_result_rel_timeout = Q.store_thm("full_result_rel_timeout",
+  `full_result_rel (Rerr(Rabort Rtimeout_error),x) (r,y) ⇒ r = Rerr (Rabort Rtimeout_error)`,
+  rw[full_result_rel_def] >>
+  Cases_on`ra`>> fs[clos_relationTheory.res_rel_rw]>>
+  rw[] >> fs[] >> rw[] >>
+  fs[clos_relationTheory.res_rel_rw]>>
+  rw[] >> fs[] >> rw[] >> fs[]);
+
+val full_result_rel_ffi = Q.store_thm("full_result_rel_ffi",
+  `r ≠ Rerr (Rabort Rtype_error) ⇒
+   full_result_rel (r,s) (r1,s1) ⇒ s.ffi = s1.ffi`,
+  rw[full_result_rel_def] >>
+  imp_res_tac clos_relationPropsTheory.res_rel_ffi >>
+  fs[clos_annotateProofTheory.state_rel_def,
+     clos_numberProofTheory.state_rel_def,
+     state_rel_def] >> rfs[] >>
+  first_x_assum(match_mp_tac o GSYM) >>
+  strip_tac >> rw[] >> fs[] >> rw[] >>
+  Cases_on`r`>>fs[clos_relationTheory.res_rel_rw] >>
+  Cases_on`e`>>fs[clos_relationTheory.res_rel_rw] >>
+  Cases_on`a`>>fs[clos_relationTheory.res_rel_rw]);
 
 val compile_evaluate = Q.store_thm("compile_evaluate",
   `evaluate ([e],[],s) = (r,s') ∧
@@ -3745,6 +3793,7 @@ val compile_evaluate = Q.store_thm("compile_evaluate",
     metis_tac[clos_mtiTheory.intro_multi_sing, SING_HD, SND,
               clos_numberTheory.renumber_code_locs_length,
               LENGTH, ONE] ) >>
+  first_x_assum(qspec_then`s.clock`strip_assume_tac) >>
   qspec_then`[e]`mp_tac clos_mtiProofTheory.intro_multi_correct >>
   simp[clos_relationTheory.exp_rel_def,clos_relationTheory.exec_rel_rw,clos_relationTheory.evaluate_ev_def] >>
   disch_then(fn th => last_assum(mp_tac o MATCH_MP(REWRITE_RULE[GSYM AND_IMP_INTRO]th))) >>
@@ -3778,6 +3827,7 @@ val compile_evaluate = Q.store_thm("compile_evaluate",
   disch_then(fn th => first_assum(mp_tac o MATCH_MP(REWRITE_RULE[GSYM AND_IMP_INTRO]th))) >>
   disch_then(qspec_then`[]`mp_tac) >> simp[] >>
   disch_then(qspec_then`sb.clock`mp_tac) >> simp[] >>
+  discharge_hyps_keep >- fs[clos_numberProofTheory.state_rel_def] >>
   strip_tac >>
   qmatch_assum_abbrev_tac`res_rel _ q` >>
   Cases_on`q`>>fs[markerTheory.Abbrev_def]>>pop_assum(assume_tac o SYM) >> fs[] >>
@@ -3833,6 +3883,131 @@ val compile_evaluate = Q.store_thm("compile_evaluate",
   simp[bvlSemTheory.dec_clock_def] >>
   metis_tac[clos_numberProofTheory.state_rel_def,
             clos_annotateProofTheory.state_rel_def]);
+
+val compile_semantics = Q.store_thm("compile_semantics",
+  `¬contains_App_SOME [e] ∧ every_Fn_vs_NONE [e] ∧
+   compile c e = (c',p)  ∧
+   full_state_rel (s:'ffi closSem$state) s1 ∧
+   code_installed p s1.code ∧
+   semantics [] s [e] ≠ Fail
+   ⇒
+   semantics [] s1 [Call 0 (SOME c'.start) []] =
+   semantics [] s [e]`,
+  simp[GSYM AND_IMP_INTRO] >> ntac 5 strip_tac >>
+  simp[closSemTheory.semantics_def] >>
+  IF_CASES_TAC >> fs[] >>
+  DEEP_INTRO_TAC some_intro >> simp[] >>
+  conj_tac >- (
+    qx_gen_tac`ffi` >> strip_tac >>
+    first_assum(mp_tac o MATCH_MP (REWRITE_RULE[GSYM AND_IMP_INTRO](GEN_ALL compile_evaluate))) >> simp[] >>
+    simp[GSYM PULL_FORALL] >>
+    discharge_hyps_keep >- metis_tac[FST] >>
+    imp_res_tac full_state_rel_with_clock >>
+    pop_assum(qspec_then`k`strip_assume_tac) >>
+    rpt(disch_then(fn th => first_assum(mp_tac o MATCH_MP th))) >> simp[] >>
+    strip_tac >>
+    simp[bvlSemTheory.semantics_def] >>
+    `r1 ≠ Rerr (Rabort Rtimeout_error) ∧
+     r1 ≠ Rerr (Rabort Rtype_error)` by (
+      conj_tac >>
+      strip_tac >> fs[] >>
+      imp_res_tac full_result_rel_abort ) >>
+    imp_res_tac full_result_rel_ffi >>
+    IF_CASES_TAC >> fs[] >- (
+      qmatch_assum_abbrev_tac`FST q = _` >>
+      Cases_on`q`>>fs[markerTheory.Abbrev_def] >>
+      pop_assum(assume_tac o SYM) >>
+      imp_res_tac bvlPropsTheory.evaluate_add_clock >> rfs[] >>
+      qspecl_then[`ck+k`,`k'`]strip_assume_tac LESS_EQ_CASES >>
+      fs[LESS_EQ_EXISTS] >>
+      qmatch_assum_rename_tac`_ = _ + (ex:num)` >>
+      rpt var_eq_tac >> rfs[] >>
+      rpt(first_x_assum(qspec_then`ex`mp_tac)) >>
+      simp[inc_clock_def] >>
+      fsrw_tac[ARITH_ss][]) >>
+    DEEP_INTRO_TAC some_intro >> simp[] >>
+    conj_tac >- (
+      qx_gen_tac`ffi'` >> strip_tac >>
+      imp_res_tac evaluate_add_clock >>
+      qspecl_then[`ck+k`,`k'`]strip_assume_tac LESS_EQ_CASES >>
+      fs[LESS_EQ_EXISTS] >>
+      qmatch_assum_rename_tac`_ = _ + (ex:num)` >>
+      rpt var_eq_tac >> rfs[] >>
+      rpt(first_x_assum(qspec_then`ex`mp_tac)) >>
+      simp[inc_clock_def] >>
+      fsrw_tac[ARITH_ss][]) >>
+    simp_tac(srw_ss()++QUANT_INST_ss[pair_default_qp])[] >>
+    qexists_tac`ck + k` >> simp[]) >>
+  strip_tac >>
+  simp[bvlSemTheory.semantics_def] >>
+  IF_CASES_TAC >> fs[] >- (
+    last_x_assum(qspec_then`k`strip_assume_tac) >>
+    qmatch_assum_abbrev_tac`FST q ≠ _` >>
+    Cases_on`q`>>fs[markerTheory.Abbrev_def] >>
+    pop_assum(assume_tac o SYM) >>
+    first_assum(mp_tac o MATCH_MP (REWRITE_RULE[GSYM AND_IMP_INTRO](GEN_ALL compile_evaluate))) >>
+    simp[GSYM PULL_FORALL] >>
+    imp_res_tac full_state_rel_with_clock >>
+    pop_assum(qspec_then`k`strip_assume_tac) >>
+    rpt(first_assum(match_exists_tac o concl)>>simp[]) >>
+    spose_not_then strip_assume_tac >>
+    qmatch_assum_abbrev_tac`FST q = _` >>
+    Cases_on`q`>>fs[markerTheory.Abbrev_def] >>
+    pop_assum(assume_tac o SYM) >>
+    imp_res_tac evaluate_add_clock >> rfs[] >>
+    first_x_assum(qspec_then`ck`mp_tac) >>
+    simp[inc_clock_def] >>
+    spose_not_then strip_assume_tac >> fs[] >>
+    imp_res_tac full_result_rel_abort) >>
+  DEEP_INTRO_TAC some_intro >> simp[] >>
+  conj_tac >- (
+    spose_not_then strip_assume_tac >>
+    fsrw_tac[QUANT_INST_ss[pair_default_qp]][] >>
+    last_x_assum(qspec_then`k`strip_assume_tac) >>
+    qmatch_assum_abbrev_tac`FST q = _` >>
+    Cases_on`q`>>fs[markerTheory.Abbrev_def] >>
+    pop_assum(assume_tac o SYM) >>
+    first_assum(mp_tac o MATCH_MP (REWRITE_RULE[GSYM AND_IMP_INTRO](GEN_ALL compile_evaluate))) >>
+    simp[] >>
+    imp_res_tac full_state_rel_with_clock >>
+    pop_assum(qspec_then`k`strip_assume_tac) >>
+    rpt(first_assum(match_exists_tac o concl)>>simp[]) >>
+    spose_not_then strip_assume_tac >>
+    first_x_assum(qspec_then`k`strip_assume_tac) >> rfs[] >>
+    imp_res_tac evaluate_add_clock >>
+    first_x_assum(qspec_then`ck`mp_tac) >>
+    simp[inc_clock_def] >> spose_not_then strip_assume_tac >>
+    fs[] >> imp_res_tac full_result_rel_timeout ) >>
+  strip_tac >>
+  (*
+  the below does not work because the clocks are not the same: need to first
+  reason that adding to the clock on the BVL side does not change the
+  lprefix_lub.
+
+  rpt (AP_TERM_TAC ORELSE AP_THM_TAC) >>
+  simp[FUN_EQ_THM] >> gen_tac >>
+  rpt (AP_TERM_TAC ORELSE AP_THM_TAC) >>
+  fsrw_tac[QUANT_INST_ss[pair_default_qp]][] >> rw[] >>
+  (compile_evaluate
+   |> Q.GEN`s` |> Q.SPEC`s with clock := k`
+   |> GEN_ALL |> SIMP_RULE(srw_ss()++QUANT_INST_ss[pair_default_qp])[]
+   |> Q.SPECL[`s1 with clock := k`,`s`,`k`,`e`,`c`]
+   |> mp_tac) >> simp[full_state_rel_with_clock] >>
+  rw[] >>
+  qmatch_assum_abbrev_tac`full_result_rel p1 p2` >>
+  Cases_on`p1`>>Cases_on`p2`>>fs[markerTheory.Abbrev_def] >>
+  ntac 2 (pop_assum(mp_tac o SYM)) >> ntac 2 strip_tac >> fs[] >>
+  qmatch_assum_rename_tac`full_result_rel (a1,b1) (a2,b2)` >>
+  `b1.ffi = b2.ffi` by metis_tac[full_result_rel_ffi,FST] >>
+  qmatch_abbrev_tac`_ (SND q) = _` >>
+  Cases_on`q`>>fs[markerTheory.Abbrev_def] >>
+  pop_assum(assume_tac o SYM) >>
+  qmatch_assum_rename_tac`_ = (r2,s2)` >>
+  `r2 = Rerr (Rabort Rtimeout_error)` by metis_tac[] >>
+  imp_res_tac evaluate_add_clock >>
+  last_x_assum(qspec_then`k`mp_tac) >> simp[]
+  *)
+  cheat);
 
 (* more correctness properties *)
 
